\documentclass[a4paper]{article}
\usepackage[shortlabels]{enumitem}
\usepackage{amsmath,amssymb,amsthm,amsfonts}
\newcommand{\bb}{\textbf}

\begin{document}

    \begin{center}
        \Large \textbf{8/24} \\
        \large \textit{Nathan Keough} \\
        Acknowledgements: \emph{None} \vspace{.5pc} \\ \line(1,0){300} 
        \vspace{1pc}
    \end{center} 
    
    \begin{flushleft}
        \begin{enumerate}
            \item [1.2.1]
            Suppose that $a, b, c \in \mathbb{R}$ and $a\leq b$.

            \begin{enumerate}
                \item [(a)]
                Prove that $a + c\leq b + c$. 
                \begin{proof} 
                    Let $a,b,c \in \mathbb{R}$ and $a\leq b$.
                    By the TP, $a < b$ or $a = b$.

                    \bb{Case 1} [Assume $a < b$] \\
                    By the AP, adding $c$ to both sides results in 
                        \begin{align}
                            &    a + c < b + c
                        \end{align}
                    \bb{Case 2} [Assume $a = b$] \\
                    By the AP, adding $c$ to both sides results in 
                        \begin{align}
                            &    a + c = b + c
                        \end{align}
                    
                    In either case, $a + c < b + c$ or $a + c = b + c$ \\
                    $\therefore a + c\leq b + c$.
                \end{proof}

                \item [(b)]
                If $c\geq 0$, prove that $a \cdot c\leq b \cdot  c$.
                \begin{proof}
                    Let $a,b,c \in \mathbb{R}$ and $a\leq b$.
                    By the TP, $a < b$ or $a = b$. 

                    \bb{Case 1} [Assume $a < b$] 
                        \begin{tabbing}
                            Now,\= by TP, $c > 0$ or $c = 0$. \\ \\
                            \> \bb{Case i. }\= [Assume $c > 0$] \+ \\
                            \> By MP1, multiplying both sides by $c > 0$ gives us \\
                            \> $a \cdot c < b \cdot c$ \- \\

                            \> \bb{Case ii.}\= [Assume $c = 0$] \+ \\
                            \> By MP, multiplying both sides by $c = 0$ gives us \\
                            \> $a \cdot c < b \cdot c$ \\
                            \> $a \cdot 0 < b \cdot 0$ \\
                            \> $= (0 = 0)$ \\
                        \end{tabbing}

                    \bb{Case 2} [Assume a = b] \\
                        \begin{tabbing}
                            Now,\= by TP, $c > 0$ or $c = 0$. \\ \\
                            \> \bb{Case i. }\= [Assume $c > 0$] \+ \\
                            \> By MP, multiplying both sides by $c > 0$ gives us \\
                            \> $a \cdot c = b \cdot c$ \- \\

                            \> \bb{Case ii.}\= [Assume $c = 0$] \+ \\
                            \> By MP, multiplying both sides by $c = 0$ gives us \\
                            \> $a \cdot c = b \cdot c$ \\
                            \> $a \cdot 0 = b \cdot 0$ \\
                            \> $= (0 = 0)$ \\
                        \end{tabbing}

                In both cases $a < b$ and $a = b$ with $c = 0$, we get $a \cdot c = b \cdot c$.\\
                In both cases $a < b$ and $a = b$ with $c > 0$, we get $a \cdot c < b \cdot c$.\\
                $\therefore a \cdot c\leq b \cdot  c$


                \end{proof}
            \end{enumerate}             
        \end{enumerate}
    \end{flushleft}

\end{document}