\documentclass[a4paper]{article}
\usepackage[shortlabels]{enumitem}
\usepackage{amsmath,amssymb,amsthm,amsfonts,tikz}
\newcommand{\bb}{\textbf}
\newcommand{\eps}{\epsilon}
\newcommand{\del}{\delta}
\newcommand{\real}{\mathbb{R}}
\newcommand{\nat}{\mathbb{N}}
\newcommand{\cir}[1]{\tikz[baseline]{%
    \node[anchor=base, draw, circle, inner sep=0, minimum width=1.2em]{#1};}}

\begin{document}

    \begin{center}
        \Large \textbf{11/2} \\
        \large \textit{Nathan Keough} \\
        Acknowledgements: \emph{Utilized the study session: Worked independently and checked work cooperatively with other classmates on this practice set.} \vspace{.5pc} \\ \line(1,0){300} 
        \vspace{1pc}
    \end{center} 
    
    \begin{flushleft}

        % % % % % % % % % % % % % % % % % %

        \bb{Wade Exercise 3.1.1}
        Using Definition 3.1, prove that each of the following limits exists. \\
        \begin{enumerate}[a.]
            \item $\lim\limits_{x \to 2} x^2 + 2x -5 = 3$.
            
            \begin{proof}\mbox{}\\*
                Let $f(x) = x^2 + 2x -5$ and Let $\eps > 0$. \\ 
                Set $\del = \min\left\{1, \frac{\eps}{7}\right\}$. \\
                Assume $0 < \left| x - 2 \right| < \del $. \\
                Then, 
                \begin{align*}
                    |x-2| < 1 &\implies -1 < x-2 < 1 & [\text{FTAV}]\\
                    &\implies 1 < x < 3 &\\
                    &\implies x \in (1,3) &\\
                    &\text{  Also note that } |x-2|<\frac{\eps}{7}
                \end{align*}
                Then, 
                \begin{align*}
                    |f - 3| &= |x-2||x+4| & [\text{Algebra/Factoring}]\\
                               &< |x-2|(|x|+4) &\\
                               &< \frac{\eps}{7} ((3)+4) &\\
                               &= \frac{\eps}{7} 7 &\\
                               &= \eps &.
                \end{align*}
                $\therefore f \to 3$ as $x \to 2$.
            \end{proof}

            \item $\lim\limits_{x \to 1} \frac{x^2 + x - 2}{x - 1} = 3$
            
            \begin{proof}\mbox{}\\*
                Let $f(x) = \frac{x^2 + x -2}{x-1}$ and Let $\eps > 0$. \\ 
                Set $\del = \eps$. \\
                Assume $0 < \left| x - 1 \right| < \del $. \\
                Notice $\left| x - 1 \right| < \eps$. \\
                Then, 
                \begin{align*}
                    |f - 3| &= |x+2 -3| & [\text{Substitution/Algebra}]\\
                            &= |x-1| \\
                            &< \eps.
                \end{align*}
                $\therefore f \to 3$ as $x \to 1$.
            \end{proof}

        \end{enumerate} 

    \end{flushleft}

\end{document}